open sums

tests/layeff/LowParseWriters.Compat.fst
@@ -138,3 +138,97 @@ let valid_synth_parse_sum
     LP.serialize_sum_eq ps.sum_t ps.sum_s #ps.sum_pc ps.sum_sc y
   );
 }
+
+let weaken_parse_dsum_cases_kind_strong_parser_kind
+  (s: LP.dsum { Cons? (LP.DSum?.e s) })
+  (f: (x: LP.dsum_known_key s) -> Tot (k: LP.parser_kind & LP.parser k (LP.dsum_type_of_known_tag s x)))
+  (f_strong: (x: LP.dsum_known_key s) -> Lemma ((dfst (f x)).LP.parser_kind_subkind == Some LP.ParserStrong))
+  (k' : LP.parser_kind { k'.LP.parser_kind_subkind == Some LP.ParserStrong })
+: Lemma
+  ((LP.weaken_parse_dsum_cases_kind s f k').LP.parser_kind_subkind == Some LP.ParserStrong)
+=
+  let keys : list (LP.dsum_key_type s) = List.Tot.map fst (LP.dsum_enum s) in
+  glb_list_of_strong #(LP.dsum_key_type s) (fun (x: LP.dsum_key_type s) ->
+    if List.Tot.mem x keys
+    then let (| k, _ |) = f x in k
+    else k'
+  ) (List.Tot.map fst (LP.dsum_enum s))
+  (fun x ->
+    if List.Tot.mem x keys
+    then f_strong x
+    else ()
+  )
+
+let parse_dsum_kind_strong
+  (ps: parse_dsum_t)
+: Lemma
+  ((LP.parse_dsum_kind ps.dsum_kt ps.dsum_t ps.dsum_pc ps.dsum_ku).LP.parser_kind_subkind == Some LP.ParserStrong)
+= weaken_parse_dsum_cases_kind_strong_parser_kind ps.dsum_t ps.dsum_pc (fun x -> let p = ps.dsum_pc' x in ()) ps.dsum_ku
+
+let parse_dsum
+  ps
+=
+  [@inline_let]
+  let _ = parse_dsum_kind_strong ps in
+  make_parser
+    (LP.parse_dsum ps.dsum_t ps.dsum_p ps.dsum_pc ps.dsum_pu)
+    (LP.serialize_dsum #ps.dsum_kt ps.dsum_t #ps.dsum_p ps.dsum_s ps.dsum_pc ps.dsum_sc ps.dsum_pu ps.dsum_su)
+    (LP.jump_dsum ps.dsum_t (dsnd ps.dsum_p').jumper ps.dsum_r ps.dsum_pc (fun x -> (dsnd (ps.dsum_pc' x)).jumper) (dsnd ps.dsum_pu').jumper ps.dsum_destr)
+
+let parse_maybe_enum
+  #key p e
+=
+  make_parser
+    (LP.parse_maybe_enum_key (get_parser p) e)
+    (LP.serialize_maybe_enum_key _ (get_serializer p) e)
+    (LP.jump_maybe_enum_key (dsnd p).jumper e)
+
+let valid_synth_parse_dsum_known
+  ps k
+= {
+  valid_synth_valid = (fun h b pos pos' ->
+    let sl = LP.make_slice b (B.len b) in
+    assert (LP.valid (LP.parse_maybe_enum_key ps.dsum_p (LP.dsum_enum ps.dsum_t) `LP.nondep_then` dsnd (ps.dsum_pc k)) h sl pos);
+    let (k', _) = LP.contents (LP.parse_maybe_enum_key ps.dsum_p (LP.dsum_enum ps.dsum_t) `LP.nondep_then` dsnd (ps.dsum_pc k)) h sl pos in
+    assert (k' == LP.Known k);
+    LP.valid_nondep_then h (LP.parse_maybe_enum_key ps.dsum_p (LP.dsum_enum ps.dsum_t)) (dsnd (ps.dsum_pc k)) sl pos;
+    assert (LP.valid (LP.parse_maybe_enum_key ps.dsum_p (LP.dsum_enum ps.dsum_t)) h sl pos);
+    assert (LP.contents (LP.parse_maybe_enum_key ps.dsum_p (LP.dsum_enum ps.dsum_t)) h sl pos == LP.Known k);
+    LP.valid_dsum_intro_known h ps.dsum_t ps.dsum_p ps.dsum_pc ps.dsum_pu sl pos
+  );
+  valid_synth_size = (fun x ->
+    let (k', pl) = LP.coerce (dfst (parse_maybe_enum ps.dsum_p' (LP.dsum_enum ps.dsum_t)) & dfst (ps.dsum_pc' k)) (x <: (dfst (parse_maybe_enum ps.dsum_p' (LP.dsum_enum ps.dsum_t) `star` ps.dsum_pc' k))) in
+    let y = LP.synth_dsum_case ps.dsum_t (LP.Known k) pl in
+    assert (LP.dsum_tag_of_data ps.dsum_t y == LP.Known k);
+    LP.synth_dsum_case_inverse ps.dsum_t (LP.Known k);
+    LP.synth_dsum_case_injective ps.dsum_t (LP.Known k);
+    LP.synth_injective_synth_inverse_synth_inverse_recip (LP.synth_dsum_case ps.dsum_t (LP.Known k)) (LP.synth_dsum_case_recip ps.dsum_t (LP.Known k)) ();
+    assert (LP.synth_dsum_case_recip ps.dsum_t (LP.Known k) y == pl);
+    LP.serialize_dsum_eq ps.dsum_t ps.dsum_s ps.dsum_pc ps.dsum_sc ps.dsum_pu ps.dsum_su y
+  );
+}
+
+let valid_synth_parse_dsum_unknown
+  ps
+= {
+  valid_synth_valid = (fun h b pos pos' ->
+    let sl = LP.make_slice b (B.len b) in
+    assert (LP.valid (LP.parse_maybe_enum_key ps.dsum_p (LP.dsum_enum ps.dsum_t) `LP.nondep_then` (ps.dsum_pu)) h sl pos);
+    let (k', _) = LP.contents (LP.parse_maybe_enum_key ps.dsum_p (LP.dsum_enum ps.dsum_t) `LP.nondep_then` (ps.dsum_pu)) h sl pos in
+    assert (LP.Unknown? k');
+    LP.valid_nondep_then h (LP.parse_maybe_enum_key ps.dsum_p (LP.dsum_enum ps.dsum_t)) ((ps.dsum_pu)) sl pos;
+    assert (LP.valid (LP.parse_maybe_enum_key ps.dsum_p (LP.dsum_enum ps.dsum_t)) h sl pos);
+    assert (LP.Unknown? (LP.contents (LP.parse_maybe_enum_key ps.dsum_p (LP.dsum_enum ps.dsum_t)) h sl pos));
+    LP.valid_dsum_intro_unknown h ps.dsum_t ps.dsum_p ps.dsum_pc ps.dsum_pu sl pos
+  );
+  valid_synth_size = (fun x ->
+    let (k', pl) = LP.coerce (dfst (parse_maybe_enum ps.dsum_p' (LP.dsum_enum ps.dsum_t)) & dfst (ps.dsum_pu')) (x <: (dfst (parse_maybe_enum ps.dsum_p' (LP.dsum_enum ps.dsum_t) `star` ps.dsum_pu'))) in
+    let y = LP.synth_dsum_case ps.dsum_t (k') pl in
+    assert (LP.dsum_tag_of_data ps.dsum_t y == k');
+    LP.synth_dsum_case_inverse ps.dsum_t (k');
+    LP.synth_dsum_case_injective ps.dsum_t (k');
+    LP.synth_injective_synth_inverse_synth_inverse_recip (LP.synth_dsum_case ps.dsum_t (k')) (LP.synth_dsum_case_recip ps.dsum_t (k')) ();
+    assert (LP.synth_dsum_case_recip ps.dsum_t (k') y == pl);
+    LP.serialize_dsum_eq ps.dsum_t ps.dsum_s ps.dsum_pc ps.dsum_sc ps.dsum_pu ps.dsum_su y
+  );
+}
